testdata/cue/division_expressions.cue
@@ -1,0 +1,4 @@
+div:      5 / 2
+whole:    6 / 3
+third:    1 / 3
+negative: -5 / 2
